\subsection{Diverses}
\begin{tabbing}
	xxxxxxxxxxxxxxxxxxxxxxxxxxxx \= xxxxxxxxxxxxxxxxxxxxxxxxxxxxxx \= \kill
 	$f'(z) = \lim \limits_{\Delta z \rightarrow 0} \frac{f(z + \Delta z) -
	f(z)}{\Delta z}$ \> $(a + b)^n = \sum_{k=0}^{n} \binom n k a^{n-k} \cdot b^k$ \>
	$(a \pm b)^3 =a^3 \pm  3 a^{2} b + 3 a b^2 \pm b^3 $\\ \\
	$x_{1,2} = \dfrac{-b \pm \sqrt{b^2 - 4ac}}{2a}$ \> $\binom n k = \dfrac{n!}{k!
	\cdot (n-k)!}$ \> $(a \pm b)^4 =a^4 \pm  4 a^{3} b + 6a^2b^2 \pm 4 a b^3 +
	b^4$\\
\end{tabbing}